compiler/backend/proofs/source_to_flatProofScript.sml
@@ -1486,7 +1486,7 @@ val compile_exp_correct' = Q.prove (
        ?s'_i1 r_i1.
          result_rel (LIST_REL o v_rel) (genv with v := s'_i1.globals) r r_i1 ∧
          s_rel genv.c s' s'_i1 ∧
-         flatSem$evaluate_match env_i1 s_i1 v_i1 pes_i1 err_v_i1 = (s'_i1, r_i1) ∧
+         flatProps$evaluate_match env_i1 s_i1 v_i1 pes_i1 err_v_i1 = (s'_i1, r_i1) ∧
          s_i1.globals = s'_i1.globals)`,
   ho_match_mp_tac terminationTheory.evaluate_ind >>
   srw_tac[][terminationTheory.evaluate_def, flatSemTheory.evaluate_def,compile_exp_def] >>
